Work on logic/connection with commutative insert with Martin, Victor, Alastair.

src/Fresh_Start.thy
@@ -3,7 +3,10 @@ theory
 imports
   Main
   "~~/src/HOL/Library/Monad_Syntax"
+  "~~/src/HOL/Library/Product_Lexorder"
 begin
+
+section\<open>A commutative operation (insert)\<close>
 
 type_synonym ('id, 'v) elt = "'id \<times> 'v"
 
@@ -66,8 +69,8 @@ using assms
 
 lemma insert_Nil_None:
   assumes "fst e1 \<noteq> fst e2" "i \<noteq> fst e2" "i2 \<noteq> Some (fst e1)"
-  shows "insert [] e2 i2 \<bind> (\<lambda>ys. insert ys e1 (Some i)) = None"
-using assms by (case_tac "i2") clarsimp+
+  shows   "insert [] e2 i2 \<bind> (\<lambda>ys. insert ys e1 (Some i)) = None"
+using assms by (cases "i2") clarsimp+
 
 lemma insert_insert_body_commute:
   assumes "a \<noteq> aa"
@@ -75,7 +78,8 @@ lemma insert_insert_body_commute:
           "aa \<notin> fst ` set xs"
           "fst e2 \<notin> fst ` set xs"
           "distinct (map fst xs)"
-  shows   "insert (insert_body xs (aa, ba)) e2 (Some a) = insert xs e2 (Some a) \<bind> (\<lambda>y. Some (insert_body y (aa, ba)))"
+  shows   "insert (insert_body xs (aa, ba)) e2 (Some a) =
+             insert xs e2 (Some a) \<bind> (\<lambda>y. Some (insert_body y (aa, ba)))"
 using assms
   apply(induction xs)
     apply clarsimp
@@ -84,8 +88,11 @@ using assms
   done
 
 lemma insert_commutes:
-  assumes "distinct (map fst (e1#e2#xs))" "i1 = None \<or> i1 \<noteq> Some (fst e2)" "i2 = None \<or> i2 \<noteq> Some (fst e1)"
-  shows   "do { ys \<leftarrow> insert xs e1 i1; insert ys e2 i2 } = do { ys \<leftarrow> insert xs e2 i2; insert ys e1 i1 }"
+  assumes "distinct (map fst (e1#e2#xs))"
+          "i1 = None \<or> i1 \<noteq> Some (fst e2)"
+          "i2 = None \<or> i2 \<noteq> Some (fst e1)"
+  shows   "do { ys \<leftarrow> insert xs e1 i1; insert ys e2 i2 } =
+             do { ys \<leftarrow> insert xs e2 i2; insert ys e1 i1 }"
 using assms
   apply(induction rule: insert.induct)
     apply clarsimp
@@ -179,4 +186,281 @@ lemma insert_insert':
       apply clarsimp
   done
 
+section\<open>Modal logic of networks\<close>
+
+datatype event_type
+  = Broadcast
+  | Deliver
+
+type_synonym 'a event = "nat \<times> event_type \<times> 'a"
+
+locale infinite_event_structure =
+  fixes carriers :: "nat \<Rightarrow> 'a event set"
+  fixes node_total_order :: "'a event \<Rightarrow> nat \<Rightarrow> 'a event \<Rightarrow> bool" (infix "\<sqsubset>\<^sup>_" 50)
+  fixes global_order :: "'a event \<Rightarrow> 'a event \<Rightarrow> bool" (infix "\<sqsubset>\<^sup>G" 50 )
+  assumes global_order_trans: "{e1, e2, e3} \<subseteq> (\<Union>i. carriers i) \<Longrightarrow> e1 \<sqsubset>\<^sup>G e2 \<Longrightarrow> e2 \<sqsubset>\<^sup>G e3 \<Longrightarrow> e1 \<sqsubset>\<^sup>G e3"
+  assumes global_order_irrefl: "e1 \<in> (\<Union>i. carriers i) \<Longrightarrow> \<not> (e1 \<sqsubset>\<^sup>G e1)"
+  assumes node_total_order_trans: "{e1, e2, e3} \<subseteq> carriers i \<Longrightarrow> e1 \<sqsubset>\<^sup>i e2 \<Longrightarrow> e2 \<sqsubset>\<^sup>i e3 \<Longrightarrow> e1 \<sqsubset>\<^sup>i e3"
+  assumes node_total_order_total: "{e1, e2} \<subseteq> carriers i \<Longrightarrow> e1 \<noteq> e2 \<Longrightarrow> (e1 \<sqsubset>\<^sup>i e2) \<or> (e2 \<sqsubset>\<^sup>i e1)"
+  assumes node_total_order_irrefl: "e1 \<in> carriers i \<Longrightarrow> \<not> (e1 \<sqsubset>\<^sup>i e1)"
+  assumes local_order_to_global: "{e1, e2} \<subseteq> carriers i \<Longrightarrow> e1 \<sqsubset>\<^sup>i e2 \<Longrightarrow> e1 \<sqsubset>\<^sup>G e2"
+  assumes global_order_to_local: "{e1, e2} \<subseteq> carriers i \<Longrightarrow> e1 \<sqsubset>\<^sup>G e2 \<Longrightarrow> e1 \<sqsubset>\<^sup>i e2"
+  assumes broadcast_before_delivery: "(i, Broadcast, m) \<in> carriers i \<Longrightarrow> (i, Broadcast, m) \<sqsubset>\<^sup>G (j, Deliver, m)"
+  assumes no_message_lost: "(i, Broadcast, m) \<in> carriers i \<Longrightarrow> (j, Deliver, m) \<in> carriers j"
+  assumes delivery_has_a_cause: "(i, Deliver, m) \<in> carriers i \<Longrightarrow> \<exists>j. (j, Broadcast, m) \<in> carriers j"
+  assumes carriers_message_consistent: "(j, bt, m) \<in> carriers i \<Longrightarrow> i = j"
+
+interpretation trivial_model: infinite_event_structure "\<lambda>m. {}" "\<lambda>e1 m e2. True" "\<lambda>e1 e2. True"
+  apply standard
+  apply auto
+  done
+
+interpretation non_trivial_model: infinite_event_structure
+  "\<lambda>m. if m = 0 then {(0, Broadcast, 0), (0, Deliver, 0)} else {(m, Deliver, 0)}"
+  "\<lambda>e1 m e2. m = 0 \<and> e1 = (0, Broadcast, 0) \<and> e2 = (0, Deliver, 0)"
+  "\<lambda>e1 e2. (\<exists>m. e1 = (0, Broadcast, 0) \<and> e2 = (m, Deliver, 0))"
+  apply standard
+  apply(case_tac "i = 0"; force)+
+  done
+
+datatype 'a formula
+  = True   ("\<top>" 65)
+  | False  ("\<bottom>" 65)
+  | Event  "'a event"
+  | Conjunction "'a formula" "'a formula" ("_/ and/ _"  [75,75]75)
+  | Implication "'a formula" "'a formula" ("_/ \<rightarrow>/ _"    [65,65]65)
+  | GlobalB     "'a formula"              ("\<box>\<^sup>G_"         [100]100)
+  | LocalB      "nat" "'a formula"        ("\<box>\<^sup>__"         [100,100]100)
+  | LabolgB     "'a formula"              ("\<box>\<^sup>-\<^sup>1\<^sup>,\<^sup>G_"       [100]100)
+  | LacolB      "nat" "'a formula"        ("\<box>\<^sup>-\<^sup>1\<^sup>,\<^sup>__"       [100,100]100)
+  | ExistsNode  "nat \<Rightarrow> 'a formula"       (binder "ExNode" 65)
+
+function (in infinite_event_structure) satisfaction :: "'a event \<Rightarrow> 'a formula \<Rightarrow> bool" (infix "\<Turnstile>" 55) where
+  "e \<Turnstile> \<top> = HOL.True" |
+  "e \<Turnstile> \<bottom> = HOL.False" |
+  "e \<Turnstile> Event e' = (e = e')" |
+  "e \<Turnstile> (\<phi> and \<psi>) = ((e \<Turnstile> \<phi>) \<and> (e \<Turnstile> \<psi>))" |
+  "e \<Turnstile> (\<phi> \<rightarrow> \<psi>) = ((e \<Turnstile> \<phi>) \<longrightarrow> (e \<Turnstile> \<psi>))" |
+  "e \<Turnstile> \<box>\<^sup>G \<phi> = (\<forall>e'. e \<sqsubset>\<^sup>G e' \<longrightarrow> e' \<Turnstile> \<phi>)" |
+  "e \<Turnstile> \<box>\<^sup>i \<phi> = (\<forall>e'. e \<sqsubset>\<^sup>i e' \<longrightarrow> e' \<Turnstile> \<phi>)" |
+  "e \<Turnstile> \<box>\<^sup>-\<^sup>1\<^sup>,\<^sup>G \<phi> = (\<forall>e'. e' \<sqsubset>\<^sup>G e \<longrightarrow> e' \<Turnstile> \<phi>)" |
+  "e \<Turnstile> \<box>\<^sup>-\<^sup>1\<^sup>,\<^sup>i \<phi> = (\<forall>e'. e' \<sqsubset>\<^sup>i e \<longrightarrow> e' \<Turnstile> \<phi>)" |
+  "e \<Turnstile> ExistsNode \<phi> = (\<exists>node. e \<Turnstile> \<phi> node)"
+by pat_completeness auto
+
+termination (in infinite_event_structure) satisfaction
+  sorry
+
+definition negation :: "'a formula \<Rightarrow> 'a formula" ("not/_" [100]100) where
+  "not \<phi> \<equiv> \<phi> \<rightarrow> \<bottom>"
+
+definition disjunction :: "'a formula \<Rightarrow> 'a formula \<Rightarrow> 'a formula" ("_/ or/  _" [75,75]75) where
+  "\<phi> or \<psi> \<equiv> not ((not \<phi>) and (not \<psi>))"
+
+definition globalD :: "'a formula \<Rightarrow> 'a formula" ("\<diamondop>\<^sup>G_" [100]100) where
+  "\<diamondop>\<^sup>G \<phi> \<equiv> not (\<box>\<^sup>G (not \<phi>))"
+
+definition localD :: "nat \<Rightarrow> 'a formula \<Rightarrow> 'a formula" ("\<diamondop>\<^sup>__" [100,100]100) where
+  "\<diamondop>\<^sup>i \<phi> \<equiv> not (\<box>\<^sup>i (not \<phi>))"
+
+lemma (in infinite_event_structure) negation_satisfaction:
+  shows "(e \<Turnstile> not \<phi>) = (\<not> (e \<Turnstile> \<phi>))"
+by(simp add: negation_def)
+
+definition (in infinite_event_structure) validity :: "'a formula \<Rightarrow> bool" ("\<Turnstile>/_" [55]55) where
+  "\<Turnstile> \<phi> \<equiv> \<forall>e \<in> (\<Union>i. carriers i). e \<Turnstile> \<phi>"
+
+lemma (in infinite_event_structure) S4_global_transitivity:
+  shows "\<Turnstile> \<box>\<^sup>G \<box>\<^sup>G \<phi> \<rightarrow> \<box>\<^sup>G \<phi>"
+unfolding validity_def
+sorry
+
+lemma (in infinite_event_structure) all_messages_delivered:
+  shows "\<Turnstile> Event (i, Broadcast, m) \<rightarrow> \<diamondop>\<^sup>G Event (i, Deliver, m)"
+unfolding validity_def globalD_def negation_def
+  apply standard+
+  apply clarsimp
+  apply(rule broadcast_before_delivery)
+  apply(frule carriers_message_consistent)
+  apply auto
+done
+
+lemma (in infinite_event_structure) messages_delivered_once:
+  shows "\<Turnstile> Event (i, Deliver, m) \<rightarrow> \<box>\<^sup>i not (Event (i, Deliver, m))"
+unfolding validity_def negation_def
+  apply standard+
+  apply clarsimp
+  apply(rule notE[OF node_total_order_irrefl], assumption)
+  apply(frule carriers_message_consistent)
+  apply auto
+done
+
+section\<open>Network events to...\<close>
+
+type_synonym lamport = "nat \<times> nat"
+
+datatype 'v operation
+  = Insert "lamport" "'v" "lamport option"
+
+definition next_lamport :: "(lamport, 'v) elt list \<Rightarrow> nat \<Rightarrow> lamport" where
+  "next_lamport xs node_name \<equiv>
+     let ss = fst ` fst ` set xs in
+       if ss = {} then
+         (node_name, 0)
+       else
+         (node_name, Suc (Max ss))"
+
+inductive possible_broadcasts :: "(lamport, 'v) elt list \<Rightarrow> nat \<Rightarrow> 'v operation event \<Rightarrow> bool" where
+  possible_broadcasts_Nil [intro!]: "\<lbrakk> next_lamport ([]::(lamport,'v) elt list) node_name = next \<rbrakk> \<Longrightarrow> possible_broadcasts [] node_name (node_name, Broadcast, (Insert next v None))" |
+  possible_broadcasts_Cons_tail [intro!]: "\<lbrakk> possible_broadcasts xs node_name tail \<rbrakk> \<Longrightarrow> possible_broadcasts (x#xs) node_name tail" |
+  possible_broadcasts_Cons_head [intro!]: "\<lbrakk> next_lamport xs node_name = next; (node_name, Broadcast, Insert next v (Some i)) = oper \<rbrakk> \<Longrightarrow> possible_broadcasts ((i,_)#xs) node_name oper"
+
+definition interpret_delivery :: "(lamport, 'v) elt list \<Rightarrow> 'v operation \<rightharpoonup> (lamport, 'v) elt list" where
+  "interpret_delivery xs oper \<equiv>
+     case oper of
+       Insert i v pos \<Rightarrow> insert xs (i, v) pos"
+
+inductive node_state_evolution :: "(lamport, 'a) elt list \<Rightarrow> nat \<Rightarrow> 'a operation event \<Rightarrow> (lamport, 'a) elt list \<Rightarrow> bool" where
+  "\<lbrakk> interpret_delivery xs oper = Some ys \<rbrakk> \<Longrightarrow> node_state_evolution xs node_name (node_name, Deliver, oper) ys" |
+  "\<lbrakk> possible_broadcasts xs node_name ev \<rbrakk> \<Longrightarrow> node_state_evolution xs node_name ev xs"
+
+inductive (in node_state_evolution' :: "(lamport, 'a) elt list \<Rightarrow> 'a operation event set \<Rightarrow> (lamport, 'a) elt list \<Rightarrow> bool" where
+  "node_state_evolution' [] {} []" |
+  "\<lbrakk> node_state_evolution' xs es ys"
+
+locale infinite_stateful_network = infinite_event_structure +
+  fixes states :: "nat \<Rightarrow> (lamport, 'a) elt list"
+  
+
 end
+
+section\<open>Modal logic of networks\<close>
+
+datatype 'a action
+  = Broadcast "'a"
+  | Deliver   "'a"
+
+datatype 'a formula
+  = True   ("\<top>" 65)
+  | False  ("\<bottom>" 65)
+  | Conjunction "'a formula" "'a formula" ("_/ &/  _" [75,75]75)
+  | Implication "'a formula" "'a formula" ("_/ \<rightarrow>/ _" [65,65]65)
+  | Atomic "nat" "'a action"
+  | Diamond "'a formula"                  ("\<diamondop>/ _" [85]85)
+  | Dnomaid "'a formula"                 ("\<diamondop>\<^sup>-\<^sup>1/ _" [85]85)
+  | Box "'a formula"                      ("\<box>/ _" [85]85)
+  | Xob "'a formula"                     ("\<box>\<^sup>-\<^sup>1/ _" [85]85)
+
+syntax
+  Broadcast_syntax :: "nat \<Rightarrow> 'a \<Rightarrow> 'a formula" ("\<B>/_/_" [85,85]85)
+  Deliver_syntax   :: "nat \<Rightarrow> 'a \<Rightarrow> 'a formula" ("\<D>/_/_" [85,85]85)
+
+translations
+  "\<B> node msg" \<rightleftharpoons> "CONST Atomic node (CONST Broadcast msg)"
+  "\<D> node msg" \<rightleftharpoons> "CONST Atomic node (CONST Deliver msg)"
+
+fun quantN :: "nat \<Rightarrow> (nat \<Rightarrow> 'a formula) \<Rightarrow> ('a formula \<Rightarrow> 'a formula \<Rightarrow> 'a formula) \<Rightarrow> 'a formula \<Rightarrow> 'a formula" where
+  "quantN 0       f j e = e" |
+  "quantN (Suc m) f j e = j (f m) (quantN m f j e)"
+
+fun satisfaction :: "(nat \<Rightarrow> 'a action \<times> nat) \<times> nat \<Rightarrow> 'a formula \<Rightarrow> bool" ("_/ \<Turnstile>/ _" [65,65]65) where
+  "(\<M>, a) \<Turnstile> \<top>      = HOL.True" |
+  "(\<M>, a) \<Turnstile> \<bottom>     = HOL.False" |
+  "(\<M>, a) \<Turnstile> \<phi> & \<psi> = ((\<M>, a) \<Turnstile> \<phi> \<and> (\<M>, a) \<Turnstile> \<psi>)" |
+  "(\<M>, a) \<Turnstile> \<phi> \<rightarrow> \<psi> = ((\<M>, a) \<Turnstile> \<phi> \<longrightarrow> (\<M>, a) \<Turnstile> \<psi>)" |
+  "(\<M>, a) \<Turnstile> \<diamondop> \<phi> = (\<exists>a'. a < a' \<and> (\<M>, a') \<Turnstile> \<phi>)" |
+  "(\<M>, a) \<Turnstile> \<box> \<phi> = (\<forall>a'. a < a' \<longrightarrow> (\<M>, a') \<Turnstile> \<phi>)" |
+  "(\<M>, a) \<Turnstile> \<diamondop>\<^sup>-\<^sup>1 \<phi> = (\<exists>a'. a' < a \<and> (\<M>, a') \<Turnstile> \<phi>)" |
+  "(\<M>, a) \<Turnstile> \<box>\<^sup>-\<^sup>1 \<phi> = (\<forall>a'. a' < a \<longrightarrow> (\<M>, a') \<Turnstile> \<phi>)" |
+  "(\<M>, a) \<Turnstile> Atomic node action = (\<M> a = (action, node))"
+
+definition Negation :: "'a formula \<Rightarrow> 'a formula" ("not/ _" [85]85) where
+  "Negation \<phi> \<equiv> \<phi> \<rightarrow> \<bottom>"
+
+definition Disjunction :: "'a formula \<Rightarrow> 'a formula \<Rightarrow> 'a formula" ("_/ orelse/ _" [75,75]75) where
+  "\<phi> orelse \<psi> \<equiv> not ((not \<phi>) & (not \<psi>))"
+
+lemma Negation_satisfaction:
+  shows "\<M> \<Turnstile> not \<phi> = (\<not> (\<M> \<Turnstile> \<phi>))"
+unfolding Negation_def by (cases "\<M>", simp)
+
+lemma Diamond_Box_deMorgan1:
+  shows "\<M> \<Turnstile> not \<diamondop> \<phi> = \<M> \<Turnstile> \<box> not \<phi>"
+unfolding Negation_def by (cases "\<M>", simp)
+
+lemma Diamond_Box_deMorgan2:
+  shows "\<M> \<Turnstile> not \<box> \<phi> = \<M> \<Turnstile> \<diamondop> not \<phi>"
+unfolding Negation_def by (cases "\<M>", simp)
+
+lemma Dnomaid_Xob_deMorgan1:
+  shows "\<M> \<Turnstile> not \<diamondop>\<^sup>-\<^sup>1 \<phi> = \<M> \<Turnstile> \<box>\<^sup>-\<^sup>1 not \<phi>"
+unfolding Negation_def by (cases "\<M>", simp)
+
+lemma Dnomaid_Xob_deMorgan2:
+  shows "\<M> \<Turnstile> not \<box>\<^sup>-\<^sup>1 \<phi> = \<M> \<Turnstile> \<diamondop>\<^sup>-\<^sup>1 not \<phi>"
+unfolding Negation_def by (cases "\<M>", simp)
+
+lemma Disjunction_Conjunction_deMorgan1:
+  shows "\<M> \<Turnstile> not (\<phi> orelse \<psi>) = \<M> \<Turnstile> (not \<phi>) & (not \<psi>)"
+unfolding Disjunction_def Negation_def by (cases "\<M>", simp)
+
+lemma Disjunction_Conjunction_deMorgan2:
+  shows "\<M> \<Turnstile> not (\<phi> & \<psi>) = \<M> \<Turnstile> (not \<phi>) orelse (not \<psi>)"
+unfolding Disjunction_def Negation_def by (cases "\<M>", simp)
+
+definition valid :: "'a formula \<Rightarrow> bool" ("\<Turnstile>/ _" [50]50) where
+  "\<Turnstile> \<phi> \<equiv> \<forall>\<M>. \<M> \<Turnstile> \<phi>"
+
+locale fixed_nodes =
+  fixes node_count :: "nat"
+
+definition (in fixed_nodes) exists :: "(nat \<Rightarrow> 'a formula) \<Rightarrow> 'a formula" (binder "Ex" 55) where
+  "exists f \<equiv> quantN node_count f Disjunction False"
+
+definition (in fixed_nodes) forall :: "(nat \<Rightarrow> 'a formula) \<Rightarrow> 'a formula" (binder "All" 55) where
+  "forall f \<equiv> quantN node_count f Conjunction True"
+
+locale network = fixed_nodes +
+  fixes R :: "'a \<Rightarrow> 'a \<Rightarrow> bool"
+  assumes all_messages_delivered: "\<And>p::nat. \<And>m::'a. \<Turnstile> (\<B> p m) \<rightarrow> \<diamondop> (\<D> p m)"
+  and messages_are_unique: "\<And>p::nat. \<And>m::'a. \<Turnstile> (\<D> p m) \<rightarrow> \<box> not (\<D> p m)"
+  and no_out_thin_air: "\<And>p::nat. \<And>m::'a. \<Turnstile> \<D> p m \<rightarrow> (Ex q. (\<diamondop>\<^sup>-\<^sup>1 (\<B> q m)))"
+  and no_message_lost: "\<And>p::nat. \<And>m::'a. \<Turnstile> (\<D> p m) \<rightarrow> (All q. ((\<diamondop> (\<D> q m)) orelse (\<diamondop>\<^sup>-\<^sup>1 (\<D> q m))))"
+  and causal_delivery: "\<And>p::nat. \<And>m1 m2::'a. R m1 m2 \<Longrightarrow> \<Turnstile> (\<D> p m2) \<rightarrow> \<diamondop>\<^sup>-\<^sup>1 (\<D> p m1)"
+
+lemma (in network) All_elim:
+  assumes "\<Turnstile> All p. f p"
+  shows   "\<And>p. p < node_count \<Longrightarrow> \<Turnstile> f p"
+using assms unfolding forall_def valid_def
+  apply clarsimp
+  apply(induction node_count; clarsimp)
+  apply(subgoal_tac "p = node_count \<or> p < node_count")
+  apply force+
+done
+
+lemma (in network) All_intro:
+  assumes "\<And>p. p < node_count \<Longrightarrow> \<Turnstile> f p"
+  shows   "\<Turnstile> All p. f p"
+using assms unfolding forall_def valid_def
+  apply clarsimp
+  apply(induction node_count; clarsimp)
+done
+
+lemma (in network) Implication_intro:
+  assumes "\<Turnstile> p \<Longrightarrow> \<Turnstile> q"
+  shows   "\<Turnstile> p \<rightarrow> q"
+using assms unfolding valid_def
+  apply simp
+  apply standard+
+  
+
+lemma (in network)
+  shows "\<Turnstile> \<B> p m \<rightarrow> (All q. \<diamondop> (D q m))"
+unfolding valid_def
+  apply standard+
+  
+
+section\<open>Modelling the network\<close>
+
+locale network =
+  fixes node_count :: "nat"
